add scala example

example/buildSrc/src/main/kotlin/Dependencies.kt
@@ -1,0 +1,5 @@
+//
+//object Libs {
+//    const val kotlinStdlib = "org.jetbrains.kotlin:kotlin-stdlib-jdk8:1.4.32"
+////     Add other libraries here
+//}
