example/buildSrc/src/main/kotlin/Versions.kt
@@ -1,0 +1,58 @@
+import org.gradle.api.JavaVersion
+import org.gradle.api.Project
+
+class Versions(private val rootProject: Project) {
+
+    // TODO : how to group them?
+    val rootGroup = rootProject.properties["rootGroup"]?.toString() ?: "ai.acyclic"
+
+    val rootID = rootProject.properties["rootID"]?.toString() ?: "scaffold"
+
+    val rootGroupID = "$rootGroup.$rootID"
+
+    val rootV = rootProject.properties["rootVersion"]?.toString() ?: "1.0.0-SNAPSHOT"
+    val rootVMajor = rootV.removeSuffix("-SNAPSHOT")
+
+    inner class Scala {
+        val group: String = rootProject.properties["scalaGroup"]?.toString() ?: "org.scala-lang"
+
+        val v: String = rootProject.properties["scalaVersion"].toString()
+        protected val vParts: List<String> = v.split('.').also { parts ->
+            require(parts.size == 3) { "Scala version must be in format 'X.Y.Z' but was: $v" }
+        }
+
+        val majorV: String = vParts[0]
+        val binaryV: String = vParts.subList(0, 2).joinToString(".")
+        val patchV: String = vParts[2]
+
+        val artifactSuffix = run {
+            if (majorV == "3") majorV
+            else binaryV
+        }
+    }
+
+    val scala: Scala by lazy { Scala() }
+
+    val javaVersion = rootProject.properties["javaVersion"]?.toString()?.let { JavaVersion.toVersion(it) }
+        ?: JavaVersion.VERSION_17
+
+    val jvmTarget = javaVersion
+
+    val scalaTestV = "3.2.19"
+    val splainV: String = rootProject.properties["splainVersion"]?.toString() ?: ""
+
+    val scalajsV: String? = rootProject.properties.get("scalaJSVersion")?.toString()
+
+
+    inner class Spark {
+
+        val v: String = rootProject.properties["sparkVersion"].toString()
+        protected val vParts: List<String> = v.split('.')
+
+        val majorV: String = vParts[0]
+        val binaryV: String = vParts.subList(0, 2).joinToString(".")
+        val patchV: String = vParts[2]
+    }
+
+    val spark: Spark by lazy { Spark() }
+}
