Lp2lc/Active/Dot_top_bot/Proof.lean
@@ -285,4 +285,651 @@ theorem subst_undo_trm_val_def_defs : ∀ (x y : Var),
   -- TODO
   sorry
 
+-- Further substitution lemmas (undo/idempotence) and label invariants
+
+theorem subst_typ_undo (x y : Var) (T : typ) :
+  y ∉ fv_typ T → subst_typ y x (subst_typ x y T) = T := by
+  -- TODO
+  sorry
+
+theorem subst_trm_undo (x y : Var) (t : trm) :
+  y ∉ fv_trm t → subst_trm y x (subst_trm x y t) = t := by
+  -- TODO
+  sorry
+
+theorem subst_idempotent_avar (x y : Var) :
+  (∀ a : avar, subst_avar x y (subst_avar x y a) = subst_avar x y a) := by
+  -- TODO
+  sorry
+
+theorem subst_idempotent_typ_dec (x y : Var) :
+  (∀ T : typ, subst_typ x y (subst_typ x y T) = subst_typ x y T) ∧
+  (∀ D : dec, subst_dec x y (subst_dec x y D) = subst_dec x y D) := by
+  -- TODO
+  sorry
+
+theorem subst_idempotent_trm_val_def_defs (x y : Var) :
+  (∀ t : trm, subst_trm x y (subst_trm x y t) = subst_trm x y t) ∧
+  (∀ v : val, subst_val x y (subst_val x y v) = subst_val x y v) ∧
+  (∀ d : defn, subst_def x y (subst_def x y d) = subst_def x y d) ∧
+  (∀ ds : defs, subst_defs x y (subst_defs x y ds) = subst_defs x y ds) := by
+  -- TODO
+  sorry
+
+theorem subst_typ_idempotent (x y : Var) (T : typ) :
+  subst_typ x y (subst_typ x y T) = subst_typ x y T := by
+  -- TODO
+  sorry
+
+theorem subst_trm_idempotent (x y : Var) (t : trm) :
+  subst_trm x y (subst_trm x y t) = subst_trm x y t := by
+  -- TODO
+  sorry
+
+theorem subst_label_of_dec (x y : Var) (D : dec) :
+  label_of_dec D = label_of_dec (subst_dec x y D) := by
+  -- TODO
+  sorry
+
+theorem subst_label_of_def (x y : Var) (d : defn) :
+  label_of_def d = label_of_def (subst_def x y d) := by
+  -- TODO
+  sorry
+
+theorem subst_defs_hasnt (x y : Var) (l : label) (ds : defs) :
+  defs_hasnt ds l → defs_hasnt (subst_defs x y ds) l := by
+  -- TODO
+  sorry
+
+-- ######################################################################
+-- Substitution principle (statements)
+
+theorem subst_rules (y : Var) (S : typ) :
+  (∀ m1 m2 G t T, ty_trm m1 m2 G t T → ∀ G1 G2 x,
+     G = G1 ++ ((x, S) :: G2) →
+     Lp2lc.Active.ok (G1 ++ ((x, S) :: G2)) →
+     y ∉ fv_ctx_types G1 →
+     ty_trm ty_general sub_general (G1 ++ subst_ctx x y G2) (trm.trm_var (avar.avar_f y)) (subst_typ x y S) →
+     m1 = ty_general → m2 = sub_general →
+     ty_trm m1 m2 (G1 ++ subst_ctx x y G2) (subst_trm x y t) (subst_typ x y T)) ∧
+  (∀ G d D, ty_def G d D → ∀ G1 G2 x,
+     G = G1 ++ ((x, S) :: G2) →
+     Lp2lc.Active.ok (G1 ++ ((x, S) :: G2)) →
+     y ∉ fv_ctx_types G1 →
+     ty_trm ty_general sub_general (G1 ++ subst_ctx x y G2) (trm.trm_var (avar.avar_f y)) (subst_typ x y S) →
+     ty_def (G1 ++ subst_ctx x y G2) (subst_def x y d) (subst_dec x y D)) ∧
+  (∀ G ds T, ty_defs G ds T → ∀ G1 G2 x,
+     G = G1 ++ ((x, S) :: G2) →
+     Lp2lc.Active.ok (G1 ++ ((x, S) :: G2)) →
+     y ∉ fv_ctx_types G1 →
+     ty_trm ty_general sub_general (G1 ++ subst_ctx x y G2) (trm.trm_var (avar.avar_f y)) (subst_typ x y S) →
+     ty_defs (G1 ++ subst_ctx x y G2) (subst_defs x y ds) (subst_typ x y T)) ∧
+  (∀ m1 m2 G T U, subtyp m1 m2 G T U → ∀ G1 G2 x,
+     G = G1 ++ ((x, S) :: G2) →
+     Lp2lc.Active.ok (G1 ++ ((x, S) :: G2)) →
+     y ∉ fv_ctx_types G1 →
+     ty_trm ty_general sub_general (G1 ++ subst_ctx x y G2) (trm.trm_var (avar.avar_f y)) (subst_typ x y S) →
+     m1 = ty_general → m2 = sub_general →
+     subtyp m1 m2 (G1 ++ subst_ctx x y G2) (subst_typ x y T) (subst_typ x y U)) := by
+  -- TODO
+  sorry
+
+theorem subst_ty_trm (y : Var) (S : typ) (G : ctx) (x : Var) (t : trm) (T : typ) :
+  ty_trm ty_general sub_general (G ++ [(x, S)]) t T →
+  Lp2lc.Active.ok (G ++ [(x, S)]) →
+  y ∉ fv_ctx_types G →
+  ty_trm ty_general sub_general G (trm.trm_var (avar.avar_f y)) (subst_typ x y S) →
+  ty_trm ty_general sub_general G (subst_trm x y t) (subst_typ x y T) := by
+  -- TODO
+  sorry
+
+theorem subst_ty_defs (y : Var) (S : typ) (G : ctx) (x : Var) (ds : defs) (T : typ) :
+  ty_defs (G ++ [(x, S)]) ds T →
+  Lp2lc.Active.ok (G ++ [(x, S)]) →
+  y ∉ fv_ctx_types G →
+  ty_trm ty_general sub_general G (trm.trm_var (avar.avar_f y)) (subst_typ x y S) →
+  ty_defs G (subst_defs x y ds) (subst_typ x y T) := by
+  -- TODO
+  sorry
+
+-- ######################################################################
+-- Some lemmas (statements)
+
+theorem corresponding_types (G : ctx) (s : sto) (x : Var) (T : typ) :
+  wf_sto G s → Env.binds x T G →
+  ((∃ S U t, Env.binds x (val.val_lambda S t) s ∧
+             ty_trm ty_precise sub_general G (trm.trm_val (val.val_lambda S t)) (typ.typ_all S U) ∧
+             T = typ.typ_all S U)
+   ∨ (∃ S ds, Env.binds x (val.val_new S ds) s ∧
+              ty_trm ty_precise sub_general G (trm.trm_val (val.val_new S ds)) (typ.typ_bnd S) ∧
+              T = typ.typ_bnd S)) := by
+  -- TODO
+  sorry
+
+theorem unique_rec_subtyping (G : ctx) (S T : typ) :
+  subtyp ty_precise sub_general G (typ.typ_bnd S) T → T = typ.typ_bnd S := by
+  -- TODO
+  sorry
+
+theorem unique_all_subtyping (G : ctx) (S U T : typ) :
+  subtyp ty_precise sub_general G (typ.typ_all S U) T → T = typ.typ_all S U := by
+  -- TODO
+  sorry
+
+theorem unique_lambda_typing (G : ctx) (x : Var) (S U T : typ) :
+  Env.binds x (typ.typ_all S U) G →
+  ty_trm ty_precise sub_general G (trm.trm_var (avar.avar_f x)) T →
+  T = typ.typ_all S U := by
+  -- TODO
+  sorry
+
+theorem lambda_not_rcd (G : ctx) (x : Var) (S U : typ) (A : typ_label) (T : typ) :
+  Env.binds x (typ.typ_all S U) G →
+  ty_trm ty_precise sub_general G (trm.trm_var (avar.avar_f x)) (typ.typ_rcd (dec.dec_typ A T T)) → False := by
+  -- TODO
+  sorry
+
+-- Record opening/label preservation
+
+theorem open_dec_preserves_label (D : dec) (x : Var) (i : Nat) :
+  label_of_dec D = label_of_dec (open_rec_dec i x D) := by
+  -- TODO
+  sorry
+
+theorem open_record_dec (D : dec) (x : Var) :
+  record_dec D → record_dec (open_dec x D) := by
+  -- TODO
+  sorry
+
+theorem open_record_typ (T : typ) (x : Var) (ls : Finset label) :
+  record_typ T ls → record_typ (open_typ x T) ls := by
+  -- TODO
+  sorry
+
+theorem open_eq_avar (x : Var) (i : Nat) (a1 a2 : avar) :
+  x ∉ fv_avar a1 → x ∉ fv_avar a2 →
+  open_rec_avar i x a1 = open_rec_avar i x a2 → a1 = a2 := by
+  -- TODO
+  sorry
+
+theorem open_eq_typ_dec (x : Var) :
+  (∀ T1 : typ, x ∉ fv_typ T1 → ∀ T2 : typ, x ∉ fv_typ T2 → ∀ i : Nat,
+     open_rec_typ i x T1 = open_rec_typ i x T2 → T1 = T2) ∧
+  (∀ D1 : dec, x ∉ fv_dec D1 → ∀ D2 : dec, x ∉ fv_dec D2 → ∀ i : Nat,
+     open_rec_dec i x D1 = open_rec_dec i x D2 → D1 = D2) := by
+  -- TODO
+  sorry
+
+theorem open_eq_typ (x : Var) (i : Nat) (T1 T2 : typ) :
+  x ∉ fv_typ T1 → x ∉ fv_typ T2 →
+  open_rec_typ i x T1 = open_rec_typ i x T2 → T1 = T2 := by
+  -- TODO
+  sorry
+
+theorem open_record_dec_rev (D : dec) (x : Var) :
+  x ∉ fv_dec D → record_dec (open_dec x D) → record_dec D := by
+  -- TODO
+  sorry
+
+theorem open_record_typ_rev (T : typ) (x : Var) (ls : Finset label) :
+  x ∉ fv_typ T → record_typ (open_typ x T) ls → record_typ T ls := by
+  -- TODO
+  sorry
+
+theorem open_record_type (T : typ) (x : Var) :
+  record_type T → record_type (open_typ x T) := by
+  -- TODO
+  sorry
+
+theorem open_record_type_rev (T : typ) (x : Var) :
+  x ∉ fv_typ T → record_type (open_typ x T) → record_type T := by
+  -- TODO
+  sorry
+
+theorem label_same_typing (G : ctx) (d : defn) (D : dec) :
+  ty_def G d D → label_of_def d = label_of_dec D := by
+  -- TODO
+  sorry
+
+theorem record_defs_typing_rec (G : ctx) (ds : defs) (S : typ) :
+  ty_defs G ds S → ∃ ls, record_typ S ls ∧ ∀ l, l ∉ ls ↔ defs_hasnt ds l := by
+  -- TODO
+  sorry
+
+theorem record_defs_typing (G : ctx) (ds : defs) (S : typ) :
+  ty_defs G ds S → record_type S := by
+  -- TODO
+  sorry
+
+theorem record_new_typing (G : ctx) (S : typ) (ds : defs) :
+  ty_trm ty_precise sub_general G (trm.trm_val (val.val_new S ds)) (typ.typ_bnd S) →
+  record_type S := by
+  -- TODO
+  sorry
+
+-- ######################################################################
+-- Narrowing (statements)
+
+def subenv_def := subenv -- local alias to emphasize usage
+
+theorem subenv_push (G G' : ctx) (x : Var) (T : typ) :
+  subenv_def G' G → Lp2lc.Active.ok ((x, T) :: G') → subenv_def ((x, T) :: G') ((x, T) :: G) := by
+  -- TODO
+  sorry
+
+theorem subenv_last (G : ctx) (x : Var) (S U : typ) :
+  subtyp ty_general sub_general G S U → Lp2lc.Active.ok (G ++ [(x, S)]) → subenv_def (G ++ [(x, S)]) (G ++ [(x, U)]) := by
+  -- TODO
+  sorry
+
+theorem narrow_rules :
+  (∀ m1 m2 G t T, ty_trm m1 m2 G t T → ∀ G',
+     m1 = ty_general → m2 = sub_general → Lp2lc.Active.ok G' → subenv_def G' G → ty_trm m1 m2 G' t T) ∧
+  (∀ G d D, ty_def G d D → ∀ G', Lp2lc.Active.ok G' → subenv_def G' G → ty_def G' d D) ∧
+  (∀ G ds T, ty_defs G ds T → ∀ G', Lp2lc.Active.ok G' → subenv_def G' G → ty_defs G' ds T) ∧
+  (∀ m1 m2 G S U, subtyp m1 m2 G S U → ∀ G',
+     m1 = ty_general → m2 = sub_general → Lp2lc.Active.ok G' → subenv_def G' G → subtyp m1 m2 G' S U) := by
+  -- TODO
+  sorry
+
+theorem narrow_typing (G G' : ctx) (t : trm) (T : typ) :
+  ty_trm ty_general sub_general G t T → subenv_def G' G → Lp2lc.Active.ok G' → ty_trm ty_general sub_general G' t T := by
+  -- TODO
+  sorry
+
+theorem narrow_subtyping (G G' : ctx) (S U : typ) :
+  subtyp ty_general sub_general G S U → subenv_def G' G → Lp2lc.Active.ok G' → subtyp ty_general sub_general G' S U := by
+  -- TODO
+  sorry
+
+-- ######################################################################
+-- Has-member inversions and helpers (statements)
+
+theorem has_member_rules_inv (G : ctx) (x : Var) (T : typ) (A : typ_label) (S U : typ) :
+  has_member_rules G x T A S U →
+  (T = typ.typ_rcd (dec.dec_typ A S U)) ∨
+  (∃ T1 T2, T = typ.typ_and T1 T2 ∧ (has_member G x T1 A S U ∨ has_member G x T2 A S U)) ∨
+  (∃ T', T = typ.typ_bnd T' ∧ has_member G x (open_typ x T') A S U) ∨
+  (∃ y B T', T = typ.typ_sel (avar.avar_f y) B ∧
+     ty_trm ty_precise sub_general G (trm.trm_var (avar.avar_f y)) (typ.typ_rcd (dec.dec_typ B T' T')) ∧
+     has_member G x T' A S U) ∨
+  (T = typ.typ_bot) := by
+  -- TODO
+  sorry
+
+theorem has_member_inv (G : ctx) (x : Var) (T : typ) (A : typ_label) (S U : typ) :
+  has_member G x T A S U →
+  (T = typ.typ_rcd (dec.dec_typ A S U)) ∨
+  (∃ T1 T2, T = typ.typ_and T1 T2 ∧ (has_member G x T1 A S U ∨ has_member G x T2 A S U)) ∨
+  (∃ T', T = typ.typ_bnd T' ∧ has_member G x (open_typ x T') A S U) ∨
+  (∃ y B T', T = typ.typ_sel (avar.avar_f y) B ∧
+     ty_trm ty_precise sub_general G (trm.trm_var (avar.avar_f y)) (typ.typ_rcd (dec.dec_typ B T' T')) ∧
+     has_member G x T' A S U) ∨
+  (T = typ.typ_bot) := by
+  -- TODO
+  sorry
+
+theorem has_member_covariance (G : ctx) (s : sto) (T1 T2 : typ) (x : Var)
+    (A : typ_label) (S2 U2 : typ) :
+  wf_sto G s →
+  subtyp ty_general sub_tight G T1 T2 →
+  ty_trm ty_general sub_tight G (trm.trm_var (avar.avar_f x)) T1 →
+  has_member G x T2 A S2 U2 →
+  ∃ S1 U1, has_member G x T1 A S1 U1 ∧
+           subtyp ty_general sub_tight G S2 S1 ∧
+           subtyp ty_general sub_tight G U1 U2 := by
+  -- TODO
+  sorry
+
+theorem has_member_monotonicity (G : ctx) (s : sto) (x : Var) (T0 : typ) (ds : defs)
+    (T : typ) (A : typ_label) (S U : typ) :
+  wf_sto G s →
+  Env.binds x (val.val_new T0 ds) s →
+  has_member G x T A S U →
+  ∃ T1, has_member G x (typ.typ_bnd T0) A T1 T1 ∧
+        subtyp ty_general sub_tight G S T1 ∧
+        subtyp ty_general sub_tight G T1 U := by
+  -- TODO
+  sorry
+
+-- ######################################################################
+-- Mode conversions and store-context relations (derived)
+
+theorem precise_to_general :
+  (∀ m1 m2 G t T, ty_trm m1 m2 G t T → m1 = ty_precise → m2 = sub_general → ty_trm ty_general sub_general G t T) ∧
+  (∀ m1 m2 G S U, subtyp m1 m2 G S U → m1 = ty_precise → m2 = sub_general → subtyp ty_general sub_general G S U) := by
+  -- TODO
+  sorry
+
+theorem precise_to_general_typing (G : ctx) (t : trm) (T : typ) :
+  ty_trm ty_precise sub_general G t T → ty_trm ty_general sub_general G t T := by
+  -- TODO
+  sorry
+
+theorem tight_to_general :
+  (∀ m1 m2 G t T, ty_trm m1 m2 G t T → m1 = ty_general → m2 = sub_tight → ty_trm ty_general sub_general G t T) ∧
+  (∀ m1 m2 G S U, subtyp m1 m2 G S U → m1 = ty_general → m2 = sub_tight → subtyp ty_general sub_general G S U) := by
+  -- TODO
+  sorry
+
+theorem tight_to_general_typing (G : ctx) (t : trm) (T : typ) :
+  ty_trm ty_general sub_tight G t T → ty_trm ty_general sub_general G t T := by
+  -- TODO
+  sorry
+
+theorem tight_to_general_subtyping (G : ctx) (S U : typ) :
+  subtyp ty_general sub_tight G S U → subtyp ty_general sub_general G S U := by
+  -- TODO
+  sorry
+
+theorem precise_to_tight :
+  (∀ m1 m2 G t T, ty_trm m1 m2 G t T → m1 = ty_precise → m2 = sub_general → ty_trm ty_general sub_tight G t T) ∧
+  (∀ m1 m2 G S U, subtyp m1 m2 G S U → m1 = ty_precise → m2 = sub_general → subtyp ty_general sub_tight G S U) := by
+  -- TODO
+  sorry
+
+theorem precise_to_tight_typing (G : ctx) (t : trm) (T : typ) :
+  ty_trm ty_precise sub_general G t T → ty_trm ty_general sub_tight G t T := by
+  -- TODO
+  sorry
+
+theorem general_to_tight (G0 : ctx) (s0 : sto) :
+  wf_sto G0 s0 →
+  (∀ m1 m2 G t T, ty_trm m1 m2 G t T → G = G0 → m1 = ty_general → m2 = sub_general → ty_trm ty_general sub_tight G t T) ∧
+  (∀ m1 m2 G S U, subtyp m1 m2 G S U → G = G0 → m1 = ty_general → m2 = sub_general → subtyp ty_general sub_tight G S U) := by
+  -- TODO
+  sorry
+
+theorem general_to_tight_subtyping (G : ctx) (s : sto) (S U : typ) :
+  wf_sto G s → subtyp ty_general sub_general G S U → subtyp ty_general sub_tight G S U := by
+  -- TODO
+  sorry
+
+theorem sto_binds_to_ctx_binds (G : ctx) (s : sto) (x : Var) (v : val) :
+  wf_sto G s → Env.binds x v s → ∃ S, Env.binds x S G := by
+  -- TODO
+  sorry
+
+theorem ctx_binds_to_sto_binds (G : ctx) (s : sto) (x : Var) (T : typ) :
+  wf_sto G s → Env.binds x T G → ∃ v, Env.binds x v s := by
+  -- TODO
+  sorry
+
+theorem val_new_typing (G : ctx) (s : sto) (x : Var) (T : typ) (ds : defs) :
+  wf_sto G s → Env.binds x (val.val_new T ds) s →
+  ty_trm ty_precise sub_general G (trm.trm_val (val.val_new T ds)) (typ.typ_bnd T) := by
+  -- TODO
+  sorry
+
+-- ######################################################################
+-- Record-sub lemmas (statements)
+
+theorem record_typ_sub_closed (T T' : typ) (ls : Finset label) :
+  record_sub T T' → record_typ T ls → ∃ ls', record_typ T' ls' ∧ ls' ⊆ ls := by
+  -- TODO
+  sorry
+
+theorem record_type_sub_closed (T T' : typ) :
+  record_sub T T' → record_type T → record_type T' := by
+  -- TODO
+  sorry
+
+theorem record_sub_trans (T1 T2 T3 : typ) :
+  record_sub T1 T2 → record_sub T2 T3 → record_sub T1 T3 := by
+  -- TODO
+  sorry
+
+theorem record_subtyping (G : ctx) (T T' : typ) :
+  subtyp ty_precise sub_general G T T' → record_type T → record_sub T T' := by
+  -- TODO
+  sorry
+
+theorem record_typ_sub_label_in (T : typ) (D : dec) (ls : Finset label) :
+  record_typ T ls → record_sub T (typ.typ_rcd D) → label_of_dec D ∈ ls := by
+  -- TODO
+  sorry
+
+theorem rcd_typ_eq_bounds (T : typ) (A : typ_label) (S U : typ) :
+  record_type T → record_sub T (typ.typ_rcd (dec.dec_typ A S U)) → S = U := by
+  -- TODO
+  sorry
+
+theorem unique_rcd_typ (T : typ) (A : typ_label) (T1 T2 : typ) :
+  record_type T →
+  record_sub T (typ.typ_rcd (dec.dec_typ A T1 T1)) →
+  record_sub T (typ.typ_rcd (dec.dec_typ A T2 T2)) →
+  T1 = T2 := by
+  -- TODO
+  sorry
+
+theorem record_type_sub_not_rec (S T : typ) (x : Var) :
+  record_sub (open_typ x S) (typ.typ_bnd T) → record_type S → False := by
+  -- TODO
+  sorry
+
+theorem shape_new_typing (G : ctx) (x : Var) (S T : typ) :
+  Env.binds x (typ.typ_bnd S) G → record_type S →
+  ty_trm ty_precise sub_general G (trm.trm_var (avar.avar_f x)) T →
+  T = typ.typ_bnd S ∨ record_sub (open_typ x S) T := by
+  -- TODO
+  sorry
+
+theorem unique_tight_bounds (G : ctx) (s : sto) (x : Var) (T1 T2 : typ) (A : typ_label) :
+  wf_sto G s →
+  ty_trm ty_precise sub_general G (trm.trm_var (avar.avar_f x)) (typ.typ_rcd (dec.dec_typ A T1 T1)) →
+  ty_trm ty_precise sub_general G (trm.trm_var (avar.avar_f x)) (typ.typ_rcd (dec.dec_typ A T2 T2)) →
+  T1 = T2 := by
+  -- TODO
+  sorry
+
+-- ######################################################################
+-- More record/has-member lemmas and possible types (statements)
+
+theorem record_type_new (G : ctx) (s : sto) (x : Var) (T : typ) (ds : defs) :
+  wf_sto G s → Env.binds x (val.val_new T ds) s → record_type (open_typ x T) := by
+  -- TODO
+  sorry
+
+theorem has_member_rcd_typ_sub2_mut :
+  ((∀ G x T A S U, has_member G x T A S U → record_type T →
+      (T = (typ.typ_rcd (dec.dec_typ A S U)) ∨ subtyp ty_precise sub_general G T (typ.typ_rcd (dec.dec_typ A S U)))) ∧
+   (∀ G x T A S U, has_member_rules G x T A S U → record_type T →
+      (T = (typ.typ_rcd (dec.dec_typ A S U)) ∨ subtyp ty_precise sub_general G T (typ.typ_rcd (dec.dec_typ A S U))))) := by
+  -- TODO
+  sorry
+
+theorem wf_sto_val_new_in_G (G : ctx) (s : sto) (x : Var) (T : typ) (ds : defs) :
+  wf_sto G s → Env.binds x (val.val_new T ds) s → Env.binds x (typ.typ_bnd T) G := by
+  -- TODO
+  sorry
+
+theorem tight_bound_completeness (G : ctx) (s : sto) (x : Var) (T : typ) (ds : defs)
+    (A : typ_label) (S U : typ) :
+  wf_sto G s → Env.binds x (val.val_new T ds) s →
+  ty_trm ty_general sub_tight G (trm.trm_var (avar.avar_f x)) (typ.typ_rcd (dec.dec_typ A S U)) →
+  subtyp ty_general sub_tight G (typ.typ_sel (avar.avar_f x) A) U ∧
+  subtyp ty_general sub_tight G S (typ.typ_sel (avar.avar_f x) A) := by
+  -- TODO
+  sorry
+
+theorem all_intro_inversion (G : ctx) (S : typ) (t : trm) (U : typ) :
+  ty_trm ty_precise sub_general G (trm.trm_val (val.val_lambda S t)) U → ∃ T, U = typ.typ_all S T := by
+  -- TODO
+  sorry
+
+theorem new_intro_inversion (G : ctx) (T : typ) (ds : defs) (U : typ) :
+  ty_trm ty_precise sub_general G (trm.trm_val (val.val_new T ds)) U →
+  U = typ.typ_bnd T ∧ record_type T := by
+  -- TODO
+  sorry
+
+-- Possible types closure (tight)
+
+theorem possible_types_closure_tight (G : ctx) (s : sto) (x : Var) (v : val) (T0 U0 : typ) :
+  wf_sto G s → Env.binds x v s → possible_types G x v T0 →
+  subtyp ty_general sub_tight G T0 U0 → possible_types G x v U0 := by
+  -- TODO
+  sorry
+
+-- Pieces and inversions for possible types
+
+theorem ty_defs_has (G : ctx) (ds : defs) (T : typ) (d : defn) :
+  ty_defs G ds T → defs_has ds d → record_type T → ∃ D, ty_def G d D ∧ record_sub T (typ.typ_rcd D) := by
+  -- TODO
+  sorry
+
+theorem defs_has_hasnt_neq (ds : defs) (d1 d2 : defn) :
+  defs_has ds d1 → defs_hasnt ds (label_of_def d2) → label_of_def d1 ≠ label_of_def d2 := by
+  -- TODO
+  sorry
+
+theorem record_has_ty_defs (G : ctx) (T : typ) (ds : defs) (D : dec) :
+  ty_defs G ds T → record_has T D → ∃ d, defs_has ds d ∧ ty_def G d D := by
+  -- TODO
+  sorry
+
+theorem pt_piece_rcd (G : ctx) (s : sto) (x : Var) (T : typ) (ds : defs) (d : defn) (D : dec) :
+  wf_sto G s → Env.binds x (val.val_new T ds) s → defs_has (open_defs x ds) d → ty_def G d D →
+  possible_types G x (val.val_new T ds) (typ.typ_rcd D) := by
+  -- TODO
+  sorry
+
+theorem pt_rcd_has_piece (G : ctx) (s : sto) (x : Var) (T : typ) (ds : defs) (D : dec) :
+  wf_sto G s → Env.binds x (val.val_new T ds) s → record_has (open_typ x T) D →
+  possible_types G x (val.val_new T ds) (typ.typ_rcd D) := by
+  -- TODO
+  sorry
+
+theorem pt_rcd_trm_inversion (G : ctx) (s : sto) (x : Var) (v : val) (a : trm_label) (T : typ) :
+  wf_sto G s → Env.binds x v s → possible_types G x v (typ.typ_rcd (dec.dec_trm a T)) →
+  ∃ S ds t, v = val.val_new S ds ∧ defs_has (open_defs x ds) (defn.def_trm a t) ∧ ty_trm ty_general sub_general G t T := by
+  -- TODO
+  sorry
+
+theorem pt_rcd_typ_inversion (G : ctx) (s : sto) (x : Var) (v : val) (A : typ_label) (S U : typ) :
+  wf_sto G s → Env.binds x v s → possible_types G x v (typ.typ_rcd (dec.dec_typ A S U)) →
+  ∃ T ds T', v = val.val_new T ds ∧ defs_has (open_defs x ds) (defn.def_typ A T') ∧
+    subtyp ty_general sub_general G S T' ∧ subtyp ty_general sub_general G T' U := by
+  -- TODO
+  sorry
+
+theorem record_sub_and (T T1 T2 : typ) :
+  record_type T → T = typ.typ_and T1 T2 → record_sub T T1 ∧ record_sub T T2 := by
+  -- TODO
+  sorry
+
+theorem record_sub_has (T1 T2 : typ) (D : dec) :
+  record_has T2 D → record_sub T1 T2 → record_has T1 D := by
+  -- TODO
+  sorry
+
+theorem pt_record_sub_has (G : ctx) (x : Var) (v : val) (T1 T2 : typ) :
+  (∀ D, record_has T1 D → possible_types G x v (typ.typ_rcd D)) →
+  record_sub T1 T2 →
+  (∀ D, record_has T2 D → possible_types G x v (typ.typ_rcd D)) := by
+  -- TODO
+  sorry
+
+theorem pt_has_record (G : ctx) (x : Var) (v : val) (T : typ) :
+  (∀ D, record_has T D → possible_types G x v (typ.typ_rcd D)) →
+  record_type T → possible_types G x v T := by
+  -- TODO
+  sorry
+
+theorem pt_has_sub (G : ctx) (x : Var) (v : val) (T U : typ) :
+  (∀ D, record_has T D → possible_types G x v (typ.typ_rcd D)) →
+  record_type T → record_sub T U → possible_types G x v U := by
+  -- TODO
+  sorry
+
+theorem possible_types_closure_record (G : ctx) (s : sto) (x : Var) (T : typ) (ds : defs) (U : typ) :
+  wf_sto G s → Env.binds x (val.val_new T ds) s → record_sub (open_typ x T) U → possible_types G x (val.val_new T ds) U := by
+  -- TODO
+  sorry
+
+theorem pt_and_inversion (G : ctx) (s : sto) (x : Var) (v : val) (T1 T2 : typ) :
+  wf_sto G s → Env.binds x v s → possible_types G x v (typ.typ_and T1 T2) →
+  possible_types G x v T1 ∧ possible_types G x v T2 := by
+  -- TODO
+  sorry
+
+-- Possible types completeness for values / tight / general
+
+theorem possible_types_completeness_for_values (G : ctx) (s : sto) (x : Var) (v : val) (T : typ) :
+  wf_sto G s → Env.binds x v s → ty_trm ty_precise sub_general G (trm.trm_val v) T → possible_types G x v T := by
+  -- TODO
+  sorry
+
+theorem possible_types_completeness_tight (G : ctx) (s : sto) (x : Var) (T : typ) :
+  wf_sto G s → ty_trm ty_general sub_tight G (trm.trm_var (avar.avar_f x)) T → ∃ v, Env.binds x v s ∧ possible_types G x v T := by
+  -- TODO
+  sorry
+
+theorem possible_types_completeness (G : ctx) (s : sto) (x : Var) (T : typ) :
+  wf_sto G s → ty_trm ty_general sub_general G (trm.trm_var (avar.avar_f x)) T → ∃ v, Env.binds x v s ∧ possible_types G x v T := by
+  -- TODO
+  sorry
+
+theorem possible_types_lemma (G : ctx) (s : sto) (x : Var) (v : val) (T : typ) :
+  wf_sto G s → Env.binds x v s → ty_trm ty_general sub_general G (trm.trm_var (avar.avar_f x)) T → possible_types G x v T := by
+  -- TODO
+  sorry
+
+theorem ctx_binds_to_sto_binds_typing (G : ctx) (s : sto) (x : Var) (T : typ) :
+  wf_sto G s → Env.binds x T G → ∃ v, Env.binds x v s ∧ ty_trm ty_precise sub_general G (trm.trm_val v) T := by
+  -- TODO
+  sorry
+
+-- Basic helper lemmas
+
+theorem var_new_typing (G : ctx) (s : sto) (x : Var) (T : typ) (ds : defs) :
+  wf_sto G s → Env.binds x (val.val_new T ds) s →
+  ty_trm ty_general sub_general G (trm.trm_var (avar.avar_f x)) (open_typ x T) := by
+  -- TODO
+  sorry
+
+theorem new_ty_defs (G : ctx) (s : sto) (x : Var) (T : typ) (ds : defs) :
+  wf_sto G s → Env.binds x (val.val_new T ds) s →
+  ty_defs G (open_defs x ds) (open_typ x T) := by
+  -- TODO
+  sorry
+
+theorem possible_types_closure (G : ctx) (s : sto) (x : Var) (v : val) (S T : typ) :
+  wf_sto G s → Env.binds x v s → possible_types G x v S → subtyp ty_general sub_general G S T → possible_types G x v T := by
+  -- TODO
+  sorry
+
+-- Canonical forms and safety
+
+theorem canonical_forms_1 (G : ctx) (s : sto) (x : Var) (T U : typ) :
+  wf_sto G s → ty_trm ty_general sub_general G (trm.trm_var (avar.avar_f x)) (typ.typ_all T U) →
+  ∃ (L : Vars) (T' : typ) (t : trm), Env.binds x (val.val_lambda T' t) s ∧ subtyp ty_general sub_general G T T' ∧
+            (∀ y, y ∉ L → ty_trm ty_general sub_general ((y, T) :: G) (open_trm y t) (open_typ y U)) := by
+  -- TODO
+  sorry
+
+theorem canonical_forms_2 (G : ctx) (s : sto) (x : Var) (a : trm_label) (T : typ) :
+  wf_sto G s → ty_trm ty_general sub_general G (trm.trm_var (avar.avar_f x)) (typ.typ_rcd (dec.dec_trm a T)) →
+  ∃ S ds t, Env.binds x (val.val_new S ds) s ∧ ty_defs G (open_defs x ds) (open_typ x S) ∧ defs_has (open_defs x ds) (defn.def_trm a t) ∧
+             ty_trm ty_general sub_general G t T := by
+  -- TODO
+  sorry
+
+theorem var_typing_implies_avar_f (G : ctx) (a : avar) (T : typ) :
+  ty_trm ty_general sub_general G (trm.trm_var a) T → ∃ x, a = avar.avar_f x := by
+  -- TODO
+  sorry
+
+theorem val_typing (G : ctx) (v : val) (T : typ) :
+  ty_trm ty_general sub_general G (trm.trm_val v) T →
+  ∃ T', ty_trm ty_precise sub_general G (trm.trm_val v) T' ∧ subtyp ty_general sub_general G T' T := by
+  -- TODO
+  sorry
+
+theorem safety (G : ctx) (s : sto) (t : trm) (T : typ) :
+  wf_sto G s → ty_trm ty_general sub_general G t T →
+  (normal_form t ∨ (∃ s' t' G' G'', red t s t' s' ∧ G' = G ++ G'' ∧ ty_trm ty_general sub_general G' t' T ∧ wf_sto G' s')) := by
+  -- TODO
+  sorry
+
 end Lp2lc.Active.Dot_top_bot
