example/build.gradle.kts
@@ -1,0 +1,20 @@
+buildscript {
+    repositories {
+        mavenCentral()
+    }
+    dependencies {
+        classpath("ch.epfl.scala:gradle-bloop_2.12:1.6.4") // suffix is always 2.12, weird
+    }
+}
+
+
+plugins {
+    id("ai.acyclic.scala3-conventions")
+}
+
+idea {
+
+    module {
+//        excludeDirs.add(file("latex"))
+    }
+}
