example/buildSrc/settings.gradle.kts
@@ -1,0 +1,8 @@
+rootProject.name = "buildSrc"
+
+pluginManagement {
+   repositories {
+      mavenCentral()
+      gradlePluginPortal()
+   }
+}
