example/buildSrc/src/main/kotlin/ai.acyclic.publish-conventions.gradle.kts
@@ -1,0 +1,83 @@
+import io.github.gradlenexus.publishplugin.NexusRepository
+import org.gradle.api.publish.maven.MavenPublication
+import org.gradle.kotlin.dsl.*
+
+plugins {
+
+    signing
+    `maven-publish`
+
+    id("io.github.gradle-nexus.publish-plugin")// version "1.3.0"
+}
+
+val vs = versions()
+
+val sonatypeApiUser = providers.gradleProperty("sonatypeApiUser")
+val sonatypeApiKey = providers.gradleProperty("sonatypeApiKey")
+if (sonatypeApiUser.isPresent && sonatypeApiKey.isPresent) {
+    nexusPublishing {
+        repositories {
+
+            withType<NexusRepository> {
+
+                username.set(sonatypeApiUser)
+                password.set(sonatypeApiKey)
+            }
+        }
+    }
+} else {
+    logger.warn("Sonatype API key not defined, skipping configuration of Maven Central publishing repository")
+}
+
+subprojects {
+
+    apply(plugin = "signing")
+    apply(plugin = "maven-publish")
+
+    // https://stackoverflow.com/a/66352905/1772342
+
+//    val signingKeyID = providers.gradleProperty("signing.gnupg.keyID")
+    val signingSecretKey = providers.gradleProperty("signing.gnupg.secretKey")
+    val signingKeyPassphrase = providers.gradleProperty("signing.gnupg.passphrase")
+
+    signing {
+        useGpgCmd()
+        if (signingSecretKey.isPresent) {
+            useInMemoryPgpKeys(signingSecretKey.get(), signingKeyPassphrase.get())
+//            useInMemoryPgpKeys(signingKeyID.get(), signingSecretKey.get(), signingKeyPassphrase.get())
+            sign(extensions.getByType<PublishingExtension>().publications)
+        } else {
+            logger.warn("PGP signing key not defined, skipping signing configuration")
+        }
+    }
+
+    apply(plugin = "maven-publish")
+
+    val rootID = vs.rootID
+    if (project.name.equals(rootID)) {
+        // Do nothing, root project should not be published
+    } else {
+
+        publishing {
+
+            val moduleID = getModuleID_Scala(project)
+
+            logger.info("module `${project.path}` will be published as `$moduleID`")
+
+            publications {
+                withType<MavenPublication> {
+                    artifactId = moduleID
+                    groupId = vs.rootGroupID
+                    // Lightweight Gradle Submodules use different groupID to avoid name collision
+                    //  which should be reverted when publishing
+
+                    val javaComponent = components["java"] as AdhocComponentWithVariants
+                    from(javaComponent)
+
+                    javaComponent.withVariantsFromConfiguration(configurations["testFixturesApiElements"]) { skip() }
+                    javaComponent.withVariantsFromConfiguration(configurations["testFixturesRuntimeElements"]) { skip() }
+                }
+            }
+        }
+    }
+}
