example/buildSrc/src/main/kotlin/ai.acyclic.scala-mixin.gradle.kts
@@ -1,0 +1,189 @@
+import com.github.benmanes.gradle.versions.updates.DependencyUpdatesTask
+import org.gradle.kotlin.dsl.*
+
+plugins {
+
+    scala
+    id("ai.acyclic.java-conventions")
+    id("io.github.cosmicsilence.scalafix")
+}
+
+val vs = versions()
+
+// TODO: remove after https://github.com/ben-manes/gradle-versions-plugin/issues/816 resolved
+tasks.named<DependencyUpdatesTask>("dependencyUpdates").configure {
+    filterConfigurations = Spec<Configuration> {
+        !it.name.startsWith("incrementalScalaAnalysis")
+    }
+}
+
+val scalametaV = "4.13.10"
+
+allprojects {
+
+    if (!plugins.hasPlugin("bloop")) {
+        apply(plugin = "bloop")
+        // DO NOT apply directly! In VSCode it will cause the conflict:
+        // Cannot add extension with name 'bloop', as there is an extension already registered with that name
+    }
+
+
+    apply(plugin = "scala")
+
+
+//    tasks.withType<AbstractArchiveTask> {
+//        archiveBaseName.set(getModuleID_Scala(project))
+//    }
+
+    dependencies {
+
+        testFixturesApi("org.scalatest:scalatest_${vs.scala.artifactSuffix}:${vs.scalaTestV}")
+
+        val jUnitPlatformV = "1.13.4"
+
+        testRuntimeOnly("org.junit.platform:junit-platform-engine:$jUnitPlatformV")
+        testRuntimeOnly("org.junit.platform:junit-platform-launcher:$jUnitPlatformV")
+        testRuntimeOnly("ai.acyclic.scalatestplus:junit-5-13_${vs.scala.artifactSuffix}:3.2.19.1")
+
+        // Don't delete, used for auto version upgrade
+        testImplementation("org.scalameta:scalameta_${vs.scala.artifactSuffix}:$scalametaV")
+
+    }
+
+    fun SourceSet.compileJavaWithScalaC() {
+        val moved = java.srcDirs
+
+        scala {
+            setSrcDirs(srcDirs + moved)
+        }
+        java {
+            setSrcDirs(emptyList<String>())
+        }
+    }
+
+    // scalaC will compiler both scala & java sources
+    sourceSets {
+        main { compileJavaWithScalaC() }
+        testFixtures { compileJavaWithScalaC() }
+        test { compileJavaWithScalaC() }
+    }
+
+    tasks {
+
+        withType<ScalaCompile> {
+
+            val jvmTarget = vs.jvmTarget.toString()
+
+            sourceCompatibility = jvmTarget
+            targetCompatibility = jvmTarget
+
+            scalaCompileOptions.apply {
+
+                loggingLevel = "verbose"
+
+                forkOptions.apply {
+
+                    memoryInitialSize = "1g"
+                    memoryMaximumSize = "4g"
+
+                    jvmArgs = listOf(
+                        // this may be over the top but the test code in macro & core frequently run implicit search on church encoded Nat type
+                        "-Xss256m",
+                        // circumventing Java 17 + Apache Spark test runner
+                        //
+                    )
+                }
+
+                additionalParameters.addAll(
+                    listOf(
+                        "-encoding", "UTF-8",
+                    )
+                )
+            }
+
+            apply(plugin = "io.github.cosmicsilence.scalafix")
+            scalafix {
+                semanticdb.autoConfigure.set(true)
+                semanticdb.version.set(scalametaV)
+            }
+        }
+
+        test {
+
+            minHeapSize = "1024m"
+            maxHeapSize = "4096m"
+
+            useJUnitPlatform {
+                includeEngines("scalatest")
+            }
+
+            /*
+in IDE:
+--add-opens=java.base/java.lang=ALL-UNNAMED --add-opens=java.base/java.lang.invoke=ALL-UNNAMED --add-opens=java.base/java.lang.reflect=ALL-UNNAMED --add-opens=java.base/java.io=ALL-UNNAMED --add-opens=java.base/java.net=ALL-UNNAMED --add-opens=java.base/java.nio=ALL-UNNAMED --add-opens=java.base/java.util=ALL-UNNAMED --add-opens=java.base/java.util.concurrent=ALL-UNNAMED --add-opens=java.base/java.util.concurrent.atomic=ALL-UNNAMED --add-opens=java.base/jdk.internal.ref=ALL-UNNAMED --add-opens=java.base/sun.nio.ch=ALL-UNNAMED --add-opens=java.base/sun.nio.cs=ALL-UNNAMED --add-opens=java.base/sun.security.action=ALL-UNNAMED --add-opens=java.base/sun.util.calendar=ALL-UNNAMED
+working directory:
+$MODULE_WORKING_DIR$
+             */
+            val addOpens =
+                """
+                        java.base/java.lang
+                        java.base/java.lang.invoke
+                        java.base/java.lang.reflect
+                        java.base/java.io
+                        java.base/java.net
+                        java.base/java.nio
+                        java.base/java.util
+                        java.base/java.util.concurrent
+                        java.base/java.util.concurrent.atomic
+                        java.base/jdk.internal.ref
+                        java.base/sun.nio.ch
+                        java.base/sun.nio.cs
+                        java.base/sun.security.action
+                        java.base/sun.util.calendar
+                    """.trimIndent().split("\n")
+            // from apache spark test runner
+
+            var allArgs = listOf(
+                "-Xmx2048m",  // Maximum heap size
+                "-XX:MaxMetaspaceSize=512m",  // Maximum metaspace size
+                "-XX:+HeapDumpOnOutOfMemoryError",  // Dump heap on OOM
+                "-Dfile.encoding=UTF-8",  // Set file encoding
+            )
+            for (pkg in addOpens) {
+                allArgs += "--add-opens=$pkg=ALL-UNNAMED"
+            }
+
+//                val str = allArgs.joinToString(" ")
+//                println("== [ScalaTest JVM arguments] == ${str}")
+
+            jvmArgs(allArgs)
+
+            testLogging {
+
+                events("passed", "skipped", "failed")
+//                events = setOf(org.gradle.api.tasks.testing.logging.TestLogEvent.FAILED, org.gradle.api.tasks.testing.logging.TestLogEvent.PASSED, org.gradle.api.tasks.testing.logging.TestLogEvent.SKIPPED, org.gradle.api.tasks.testing.logging.TestLogEvent.STANDARD_OUT)
+//                exceptionFormat = org.gradle.api.tasks.testing.logging.TestExceptionFormat.FULL
+                showExceptions = true
+                showCauses = true
+                showStackTraces = true
+
+//                showStandardErrors = true
+                // stdout is used for occasional manual verification
+//                showStandardStreams = true
+            }
+        }
+
+    }
+
+    idea {
+
+        module {
+
+            excludeDirs = excludeDirs + listOf(
+                file(".bloop"),
+                file(".bsp"),
+                file(".metals"),
+                file(".ammonite"),
+            )
+        }
+    }
+}
