example/buildSrc/src/main/kotlin/ai.acyclic.scala3-conventions.gradle.kts
@@ -1,0 +1,49 @@
+plugins {
+
+    id("ai.acyclic.scala-mixin")
+    id("io.github.cosmicsilence.scalafix")
+}
+
+val vs = versions()
+
+allprojects {
+
+    dependencies {
+
+        bothImpl("org.scala-lang:scala3-library_3:${vs.scala.v}")
+        bothImpl("org.scala-lang:scala3-staging_3:${vs.scala.v}")
+    }
+
+    tasks {
+
+        withType<ScalaCompile> {
+
+            scalaCompileOptions.apply {
+
+                additionalParameters.addAll(
+                    listOf(
+//                        "-verbose"
+                        "-explain",
+
+                        "-experimental",
+                        "-feature",
+
+//                        "-rewrite",
+//                        "-source:future-migration",
+                        "-source:future",
+
+//                        "-language:experimental.modularity",
+                        "-explain-cyclic",
+
+                        "-Wunused:all",// demand by scalafix
+
+//                        "-language:experimental.dependent"
+
+//                        "-verbose", // enable in case of compiler bug
+//                        "-Ydebug",
+                    )
+                )
+            }
+        }
+    }
+}
