example/settings.gradle.kts
@@ -1,0 +1,9 @@
+rootProject.name = "lp2-lc-example"
+//val versions = gradle.rootProject.versions()
+
+pluginManagement.repositories {
+    gradlePluginPortal()
+    mavenLocal()
+    mavenCentral()
+    maven("https://dl.bintray.com/kotlin/kotlin-dev")
+}
